finish exercise 3.12

Chapter 3/ASMReg0.thy
@@ -40,25 +40,24 @@ subsection "Compilation"
   
   (* The compiler takes an arithmetic expression a and produces a list of
 instructions whose execution places the value of a into register 0. 
-TODO The registers > r should be used in a
-stack-like fashion for intermediate results. *)
-fun compile :: "aexp \<Rightarrow> instr list" where
-  "compile (N n) = [LDI0 n]" |
-  "compile (V v) = [LD0 v]" |
-  "compile (Plus e\<^sub>1 e\<^sub>2) = (let
-    left = compile e\<^sub>1;
-    right = compile e\<^sub>2
-  in left @ MV0 1 @ right @ [ADD0 1])"
-  (* LDI0 val | (* register 0 is the target *) *)
-  (* LD0 vname | (* register 0 is the target *) *)
-  (* MV0 reg | (* register 0 is the source *) *)
-  (* ADD0 reg (* register 0 is the target, and an operand *) *)
-  
+The registers > r should be used in a stack-like fashion for intermediate results, the ones < r
+should be left alone. *)
+fun compile :: "aexp \<Rightarrow> reg \<Rightarrow> instr list" where
+  "compile (N n) _ = [LDI0 n]" |
+  "compile (V v) _ = [LD0 v]" |
+  "compile (Plus e\<^sub>1 e\<^sub>2) r = 
+    compile e\<^sub>1 (r+1) @ [MV0 (r+1)] @ compile e\<^sub>2 (r + 2) @ [ADD0 (r+1)]" 
+(*   "compile (Plus e\<^sub>1 e\<^sub>2) r = (
+    if r > 0
+    then compile e\<^sub>1 r @ [MV0 r] @ compile e\<^sub>2 (r + 1) @ [ADD0 r]
+    else compile e\<^sub>1 1 @ [MV0 1] @ compile e\<^sub>2 2 @ [ADD0 1])" 
+ *)
 value "compile (Plus (N 9) (N 10)) 0"
 value "exec (compile (Plus (N 9) (N 10)) 1) <> <> 1"
   
 lemma lesser_registers_unchanged:
-  "reg\<^sub>q\<^sub>u\<^sub>e\<^sub>r\<^sub>y < reg\<^sub>d\<^sub>e\<^sub>s\<^sub>t \<Longrightarrow> 
+  "reg\<^sub>q\<^sub>u\<^sub>e\<^sub>r\<^sub>y < reg\<^sub>d\<^sub>e\<^sub>s\<^sub>t \<Longrightarrow>
+   reg\<^sub>q\<^sub>u\<^sub>e\<^sub>r\<^sub>y \<noteq> 0 \<Longrightarrow> 
     (exec (compile exp reg\<^sub>d\<^sub>e\<^sub>s\<^sub>t) st rs) reg\<^sub>q\<^sub>u\<^sub>e\<^sub>r\<^sub>y = rs reg\<^sub>q\<^sub>u\<^sub>e\<^sub>r\<^sub>y"
   (* arbitrary reg\<^sub>d\<^sub>e\<^sub>s\<^sub>t is required because it changes when compiling ADD
     arbitrary rs is required because it changes when executing *)
@@ -66,12 +65,11 @@ lemma lesser_registers_unchanged:
     apply(simp_all)
   using exec_append by simp
 
-theorem compile_is_correct: "exec (compile expr reg_dest) state rs reg_dest = aval expr state"
+theorem compile_is_correct: "exec (compile expr reg_dest) state rs 0 = aval expr state"
   (* reg_dest is arbitrary because it changes during compile ADD
     rs is arbitrary because it changes during exec*)
   apply(induction expr arbitrary: reg_dest rs)
     apply(simp_all)
   using exec_append lesser_registers_unchanged by simp
-    
-  
+
 end
